almost ready to PR

test/rewrite_all.lean
@@ -7,10 +7,10 @@ structure F :=
 
 example (f : F) : f.v.val = [] :=
 begin
-perform_nth_rewrite 0 [f.p],
+  perform_nth_rewrite 0 [f.p],
 end
 
-private structure cat :=
+structure cat :=
   (O : Type)
   (H : O → O → Type)
   (i : Π o : O, H o o)
@@ -21,14 +21,12 @@ private structure cat :=
 
 open tactic
 
-set_option pp.implicit true
-private example (C : cat) (W X Y Z : C.O) (f : C.H X Y) (g : C.H W X) (h k : C.H Y Z) : C.c (C.c g f) h = C.c g (C.c f h) :=
+example (C : cat) (W X Y Z : C.O) (f : C.H X Y) (g : C.H W X) (h k : C.H Y Z) : C.c (C.c g f) h = C.c g (C.c f h) :=
 begin
- perform_nth_rewrite 0 [C.a],
+  perform_nth_rewrite 0 [C.a],
 end
 
-
-private example (C : cat) (X Y : C.O) (f : C.H X Y) : C.c f (C.i Y) = f :=
+example (C : cat) (X Y : C.O) (f : C.H X Y) : C.c f (C.i Y) = f :=
 begin
   perform_nth_rewrite 0 [C.ri],
 end
