src/tactic/rewrite_search/rewrite_all/common.lean
@@ -1,9 +1,21 @@
 import data.option.defs data.mllist
-import tactic.rewrite_search.core.data
 
 open tactic
 
-universe u
+@[derive decidable_eq]
+inductive side
+| L
+| R
+
+def side.other : side → side
+| side.L := side.R
+| side.R := side.L
+
+def side.to_string : side → string
+| side.L := "L"
+| side.R := "R"
+
+instance : has_to_string side := ⟨side.to_string⟩
 
 namespace tactic.rewrite_all
 meta structure cfg extends rewrite_cfg :=
@@ -11,16 +23,16 @@ meta structure cfg extends rewrite_cfg :=
 (discharger : tactic unit := skip)
 (simplifier : expr → tactic (expr × expr) := λ e, failed) -- FIXME this currently breaks "explanations"
 
--- rewrite_all.2, if resurrected, needs to implement this now, see TODO below:
 meta structure tracked_rewrite :=
 (exp : expr)
 (proof : tactic expr)
--- TODO perhaps make this an `option (list side)`, so that the underlying implementation
--- can not return it if it wants.
-(addr : list side)
+-- If `addr` is not provided by the underlying implementation of `rewrite_all`,
+-- `rewrite_search` will not be able to produce tactic scripts.
+(addr : option (list side))
 end tactic.rewrite_all
 
 section
+universe u
 variables {m : Type u → Type u} [monad m]
 meta def tactic.mllist.squash {α : Type u} (t : m (mllist m α)) : mllist m α :=
 (mllist.m_of_list [t]).join
