src/tactic/rewrite_search/rewrite_all/old.lean
@@ -7,7 +7,9 @@ import lib.pretty_print
 import lib.tactic
 import .common
 
-open tactic
+namespace tactic
+
+namespace rewrite_all
 
 meta def rewrite_without_new_mvars (r : expr) (e : expr) (cfg : rewrite_all.cfg := {}) : tactic (expr × expr) :=
 lock_tactic_state $ -- This makes sure that we forget everything in between rewrites; otherwise we don't correctly find everything!
@@ -134,15 +136,17 @@ def remove_adjacent_duplicates {α β} (f : α → β) [decidable_eq β] : list 
 | [x] := [x]
 | [] := []
 
+end rewrite_all
 
+open rewrite_all
 
-meta def rewrite_all (r : expr × bool) (e : expr) (cfg : rewrite_all.cfg := {}) : tactic (list (expr × expr)) :=
+meta def rewrite_all (r : expr × bool) (e : expr) (cfg : rewrite_all.cfg := {}) : tactic (list tracked_rewrite) :=
 do
    results ← rewrite_fold (rewrite_F cfg r) e [],
-   return (remove_adjacent_duplicates (λ p, p.1) results)
+   let L := (remove_adjacent_duplicates (λ p : expr × expr, p.1) results),
+   return $ L.map (λ p, ⟨p.1, pure p.2, none⟩)
 
-meta def rewrite_all_lazy (r : expr × bool) (e : expr) (cfg : rewrite_all.cfg := {}) : mllist tactic (expr × tactic expr) :=
-mllist.squash $
-do L ← rewrite_all r e cfg,
-   let L : list (expr × tactic expr) := L.map (λ p, (p.1, pure p.2)),
-   return (mllist.of_list L)
+meta def rewrite_all_lazy (r : expr × bool) (e : expr) (cfg : rewrite_all.cfg := {}) : mllist tactic tracked_rewrite :=
+mllist.squash $ mllist.of_list <$> (rewrite_all r e cfg)
+
+end tactic
